Enhance the well-formed property
A well-formed game is now also guaranteed to have a correct distribution
of cells (e.g. you can't have two `X` marks and zero `O` marks)

TicTacToe/Basic.lean
@@ -15,6 +15,16 @@ theorem vector_cons_equivalence {α} {xs : Vector α (Nat.succ n)} : xs = vector
     unfold vector_cons
     simp
 
+theorem vector_count_set {α n} {i : Fin n} {pred : α → Bool} {value : α} {xs : Vector α n} {hOld : ¬pred xs[i]} {hNew : pred value} : Vector.countP pred (Vector.set xs i value) = Vector.countP pred xs + 1 := by
+  simp at hOld
+  let hCountSet := Vector.countP_set (p := pred) (xs := xs) (a := value) i.2
+  simp [hCountSet, hNew, hOld]
+
+theorem vector_count_set_other {α n} {i : Fin n} {pred : α → Bool} {value : α} {xs : Vector α n} {hOld : ¬pred xs[i]} {hNew : ¬pred value} : Vector.countP pred (Vector.set xs i value) = Vector.countP pred xs := by
+  simp at hOld
+  let hCountSet := Vector.countP_set (p := pred) (xs := xs) (a := value) i.2
+  simp [hCountSet, hNew, hOld]
+
 theorem vector_cons_set {xs : Vector α n} {i : Fin (Nat.succ n)} : (vector_cons x xs).set i a = if hEq : i.val == 0 then vector_cons a xs else let n' := i.pred (by simp at hEq; simp [hEq]); vector_cons x (xs.set n' a) := by
   by_cases h : (i = 0)
   . simp [h, vector_cons, Vector.set]
@@ -75,6 +85,90 @@ theorem vectorSetGetUnchanged
               . simpa [h]
               . simpa [h]
 
+theorem tupToAnd {a b c d : Bool} (h : (a, b) = (c, d)) : (a = c) ∧ b = d := by grind
+
+theorem countDisjointList {xs} (hDisjoint : ∀ a, (pred1 a → ¬pred2 a) ∧ (pred2 a → ¬pred1 a)) : List.countP pred1 xs + List.countP pred2 xs = List.countP (fun x => pred1 x || pred2 x) xs := by
+  match xs with
+  | .nil => simp
+  | .cons head .nil =>
+    simp
+    match hPred : (pred1 head, pred2 head) with
+    | (true, true)   =>
+      let hDisjoint := hDisjoint head
+      simp [tupToAnd hPred] at hDisjoint
+    | (true, false)  => simp [tupToAnd hPred]
+    | (false, true)  => simp [tupToAnd hPred]
+    | (false, false) => simp [tupToAnd hPred]
+  | .cons head tail =>
+    let hRec := countDisjointList (xs := tail) hDisjoint
+    simp [List.countP_cons]
+    match hPred : (pred1 head, pred2 head) with
+    | (true, true)   =>
+      let hDisjoint := hDisjoint head
+      simp [tupToAnd hPred] at hDisjoint
+    | (true, false)  =>
+      simp [tupToAnd hPred]
+      let hAssoc := Nat.add_assoc (List.countP pred1 tail) 1 (List.countP pred2 tail)
+      let hComm := Nat.add_comm 1 (List.countP pred2 tail)
+      rw [hAssoc, hComm]
+      let hAssoc' := Nat.add_assoc (List.countP pred1 tail) (List.countP pred2 tail) 1
+      simp [← hAssoc', hRec]
+    | (false, true)  =>
+      simp [tupToAnd hPred]
+      let hAssoc := Nat.add_assoc (List.countP pred1 tail) (List.countP pred2 tail) 1
+      let hComm := Nat.add_comm 1 (List.countP pred2 tail)
+      rw [← hAssoc, hRec]
+    | (false, false) => simp [tupToAnd hPred, hRec]
+
+theorem countDisjoint {n} {pred1 pred2 : α → Bool} {xs : Vector α n} (hDisjoint : ∀ a, (pred1 a → ¬pred2 a) ∧ (pred2 a → ¬pred1 a)) : Vector.countP pred1 xs + Vector.countP pred2 xs = Vector.countP (fun x => pred1 x || pred2 x) xs := by
+  simp [← Vector.countP_toList]
+  exact countDisjointList (xs := xs.toList) hDisjoint
+
+theorem countCompleteList {pred1 pred2 : α → Bool} {xs : List α} (hDisjoint : ∀ a, pred1 a != pred2 a) (hComplete : ∀ a, pred1 a || pred2 a)
+  : List.countP pred1 xs + List.countP pred2 xs = List.length xs := by
+  match xs with
+  | .nil => simp
+  | .cons head .nil =>
+    simp
+    match hPred : (pred1 head, pred2 head) with
+    | (true, true)   =>
+      let hDisjoint := hDisjoint head
+      simp [tupToAnd hPred] at hDisjoint
+    | (true, false)  => simp [tupToAnd hPred]
+    | (false, true)  => simp [tupToAnd hPred]
+    | (false, false) =>
+      let h := hComplete head
+      simp [tupToAnd hPred] at h
+  | .cons head tail =>
+    let hRec := countCompleteList (xs := tail) hDisjoint hComplete
+    simp [List.countP_cons]
+    match hPred : (pred1 head, pred2 head) with
+    | (true, true)   =>
+      let hDisjoint := hDisjoint head
+      simp [tupToAnd hPred] at hDisjoint
+    | (true, false)  =>
+      simp [tupToAnd hPred]
+      let hAssoc := Nat.add_assoc (List.countP pred1 tail) 1 (List.countP pred2 tail)
+      let hComm := Nat.add_comm 1 (List.countP pred2 tail)
+      rw [hAssoc, hComm]
+      let hAssoc' := Nat.add_assoc (List.countP pred1 tail) (List.countP pred2 tail) 1
+      simp [← hAssoc', hRec]
+    | (false, true)  =>
+      simp [tupToAnd hPred]
+      let hAssoc := Nat.add_assoc (List.countP pred1 tail) (List.countP pred2 tail) 1
+      let hComm := Nat.add_comm 1 (List.countP pred2 tail)
+      rw [← hAssoc, hRec]
+    | (false, false) =>
+      let h := hComplete head
+      simp [tupToAnd hPred] at h
+
+theorem countComplete {pred1 pred2 : α → Bool} {xs : Vector α n} (hDisjoint : ∀ a, pred1 a != pred2 a) (hComplete : ∀ a, pred1 a || pred2 a)
+  : Vector.countP pred1 xs + Vector.countP pred2 xs = Vector.size xs := by
+  have h : Vector.size xs = xs.toList.length := by simp
+  rw [h]
+  simp only [← Vector.countP_toList]
+  exact countCompleteList (xs := xs.toList) hDisjoint hComplete
+
 -- Tic-tac-toe game
 
 inductive Player where
@@ -93,9 +187,13 @@ theorem cellNeqEmptyOccupied {player} : (Cell.Empty == Cell.Occupied player) = f
 def Board := Vector Cell 9
 def Position := Fin 9
 
+instance : Membership Cell Board := by
+  dsimp [Board]
+  infer_instance
+
 inductive GameStatus where
-  | InProgress : Player → GameStatus -- `Player` indicates who's turn it is
-  | Won : Player → GameStatus        -- `Player` indicates who won
+  | InProgress : GameStatus
+  | Won : Player → GameStatus -- `Player` indicates who won
   | Draw : GameStatus
 deriving Repr, DecidableEq
 
@@ -107,7 +205,7 @@ def emptyBoard : Board :=
   Vector.replicate 9 Cell.Empty
 
 def initialGameState : TicTacToeState :=
-  { board := emptyBoard, status := GameStatus.InProgress Player.X }
+  { board := emptyBoard, status := GameStatus.InProgress }
 
 def isEmptyPosition (board : Board) (pos : Position) : Bool := board.get pos == Cell.Empty
 
@@ -128,11 +226,10 @@ theorem switchPlayerNeg (player : Player) : ¬switchPlayer player = player := by
   | Player.X => trivial
   | Player.O => trivial
 
-def isBoardFull (board : Board) : Bool :=
-  (List.finRange 9).all (fun i =>
-    match board.get i with
-    | Cell.Empty => false
-    | Cell.Occupied _ => true)
+def isBoardFull (board : Board) : Bool := Vector.count Cell.Empty board == 0
+
+def countMarkedCells (board : Board) (player : Player) : Nat :=
+  board.countP (· == Cell.Occupied player)
 
 def checkWin (board : Board) (player : Player) : Bool :=
   let playerCell := Cell.Occupied player
@@ -149,22 +246,34 @@ def checkWin (board : Board) (player : Player) : Bool :=
   winningLines.any (fun line =>
     line.countP (fun pos => board.get pos == playerCell) >= 3)
 
+def turnNumber (state : TicTacToeState) : Nat :=
+  9 - state.board.count Cell.Empty
+
+def currentPlayer (state : TicTacToeState) : Player :=
+  if turnNumber state % 2 == 0 then Player.X else Player.O
+
 def wellFormedGame (state : TicTacToeState) : Bool :=
   match state.status with
-  | GameStatus.InProgress _ =>
+  | GameStatus.InProgress =>
       !isBoardFull state.board
       && !checkWin state.board Player.X
       && !checkWin state.board Player.O
-  | GameStatus.Won player =>
-      checkWin state.board player && !checkWin state.board (switchPlayer player)
+      && (currentPlayer state == Player.O && countMarkedCells state.board Player.O + 1 == countMarkedCells state.board Player.X || currentPlayer state == Player.X && countMarkedCells state.board Player.O == countMarkedCells state.board Player.X)
+  | GameStatus.Won victoriousPlayer =>
+      checkWin state.board victoriousPlayer
+      && !checkWin state.board (switchPlayer victoriousPlayer)
+      && (victoriousPlayer == Player.O && countMarkedCells state.board Player.O == countMarkedCells state.board Player.X || victoriousPlayer == Player.X && countMarkedCells state.board Player.O + 1 == countMarkedCells state.board Player.X)
   | GameStatus.Draw =>
       isBoardFull state.board
       && !checkWin state.board Player.X
       && !checkWin state.board Player.O
+      && countMarkedCells state.board Player.O == 4
+      && countMarkedCells state.board Player.X == 5
 
 theorem initialGameStateIsWellFormed (state : TicTacToeState) {h: state = initialGameState} : wellFormedGame state := by
   unfold initialGameState at h
-  unfold wellFormedGame
+  simp [wellFormedGame]
+
   let hStatus := congrArg (fun s => s.status) h
   simp at hStatus
   rw [hStatus]
@@ -174,25 +283,33 @@ theorem initialGameStateIsWellFormed (state : TicTacToeState) {h: state = initia
   simp at hBoard
   rw [hBoard]
 
+  have hCurrentPlayer : currentPlayer state = Player.X := by
+    simp [currentPlayer, turnNumber, hBoard, emptyBoard]
+
+  simp [hCurrentPlayer]
+
   have hGetFromEmptyBoard (i : Position) : Vector.get emptyBoard i = Cell.Empty := by
     unfold emptyBoard Vector.replicate Vector.get Vector.toArray
     simp
 
   have hBoardNotFull : isBoardFull emptyBoard = false := by
-    unfold isBoardFull
-    simp
-    refine ⟨0, ?_⟩
-    rw [hGetFromEmptyBoard (0 : Fin 9 )]
-    simp
-    trivial
+    simp [isBoardFull, emptyBoard]
 
-  have hCheckWinEmpty (p : Player) : checkWin emptyBoard p = false := by
-    unfold checkWin
-    simp [hGetFromEmptyBoard]
+  have hCheckWinEmpty (p : Player) : checkWin emptyBoard p = false := by simp [checkWin, hGetFromEmptyBoard]
 
-  simp [hCheckWinEmpty Player.X, hCheckWinEmpty Player.O, hBoardNotFull]
+  have hCheckMarkedCells (p : Player) : countMarkedCells emptyBoard p = 0 := by
+    simp [countMarkedCells, emptyBoard]
 
-def makeMove {player : Player} (state : TicTacToeState) (pos : Position) (_ : state.status = GameStatus.InProgress player) (_ : isEmptyPosition state.board pos) (_ : wellFormedGame state) : TicTacToeState :=
+  simp [
+    hCheckWinEmpty Player.X,
+    hCheckWinEmpty Player.O,
+    hBoardNotFull,
+    hCheckMarkedCells Player.X,
+    hCheckMarkedCells Player.O
+  ]
+
+def makeMove (state : TicTacToeState) (pos : Position) (_ : state.status = GameStatus.InProgress) (_ : isEmptyPosition state.board pos) (_ : wellFormedGame state) : TicTacToeState :=
+  let player := currentPlayer state
   let newBoard := state.board.set pos.val (Cell.Occupied player)
   let newStatus :=
     if checkWin newBoard player then
@@ -200,7 +317,7 @@ def makeMove {player : Player} (state : TicTacToeState) (pos : Position) (_ : st
     else if isBoardFull newBoard then
       GameStatus.Draw
     else
-      GameStatus.InProgress (switchPlayer player)
+      GameStatus.InProgress
   { board := newBoard, status := newStatus }
 
 theorem noWinWithoutOwnMove
@@ -269,66 +386,407 @@ theorem noWinWithoutOwnMove
     noCountChange hNoWin.right.right.right.right.right.right.right,
   ]
 
+theorem moveIncrementsTurnNumber
+  (state : TicTacToeState)
+  (newState : TicTacToeState)
+  (pos : Position)
+  (hIsEmpty : isEmptyPosition state.board pos)
+  (hNewBoard : newState.board = Vector.set state.board pos.val (Cell.Occupied (currentPlayer state)))
+  : turnNumber newState = turnNumber state + 1 := by
+  simp [turnNumber]
+
+  have hAtLeastOneNonEmpty : Cell.Empty ∈ state.board := by
+    simp [isEmptyPosition, Vector.get] at hIsEmpty
+    let hIsMember := Vector.getElem_mem (xs := state.board) (i := pos.val) pos.2
+    simp [hIsEmpty] at hIsMember
+    exact hIsMember
+
+  have hCount := Vector.count_pos_iff (xs := state.board) (a := Cell.Empty)
+  have hCountSet := Vector.count_set (xs := state.board) (b := Cell.Empty) (a := Cell.Occupied (currentPlayer state)) (i := pos.val) pos.2
+
+  simp [isEmptyPosition, Vector.get] at hIsEmpty
+  simp [hIsEmpty] at hCountSet
+
+  have hLemma : Vector.count Cell.Empty newState.board + 1 = Vector.count Cell.Empty state.board := by
+    simp [hNewBoard]
+    simp [hCountSet]
+    exact Nat.sub_add_cancel (hCount.mpr hAtLeastOneNonEmpty)
+
+  simp [← hLemma]
+  have hNewStateCellEmptyLemma : Vector.count Cell.Empty newState.board ≤ 8 := by
+    simp [hNewBoard, hCountSet, Vector.count_le_size]
+
+  let hNatSub := Nat.sub_add_comm hNewStateCellEmptyLemma (n := 8) (m := 1) (k := Vector.count Cell.Empty newState.board)
+  simp at hNatSub
+  exact hNatSub
+
+theorem hBoardNotFullIfCellEmpty
+  (state : TicTacToeState)
+  (pos : Position)
+  (hIsEmpty : isEmptyPosition state.board pos)
+  : ¬isBoardFull state.board := by
+  simp [isBoardFull]
+  simp [isEmptyPosition, Vector.get] at hIsEmpty
+  by_cases h : state.board.count Cell.Empty = 0
+  .
+    let hNoEmpty := state.board.not_mem_of_count_eq_zero h
+    let hPosEmpty := state.board.getElem_mem pos.2
+    simp [hIsEmpty] at hPosEmpty
+    contradiction
+  . trivial
+
+theorem cellEmptyCountOfIsEmpty (hIsEmpty : isEmptyPosition board pos) : board.count Cell.Empty ≥ 1 := by
+  simp [isEmptyPosition, Vector.get] at hIsEmpty
+  let hPosEmpty := board.getElem_mem pos.2
+  simp [hIsEmpty] at hPosEmpty
+  simp [hPosEmpty]
+
+theorem moveDecrementsEmptyCellCount
+  (state : TicTacToeState)
+  (newState : TicTacToeState)
+  (pos : Position)
+  (hIsEmpty : isEmptyPosition state.board pos)
+  (hNewBoard : newState.board = Vector.set state.board pos.val (Cell.Occupied (currentPlayer state)))
+  : newState.board.count Cell.Empty + 1 = state.board.count Cell.Empty := by
+  simp [hNewBoard]
+  let hCountSet := Vector.count_set (xs := state.board) (a := Cell.Occupied (currentPlayer state)) (b := Cell.Empty) pos.2
+  simp [hCountSet]
+
+  let hIsEmpty' := hIsEmpty
+  simp [isEmptyPosition, Vector.get] at hIsEmpty'
+  simp [hIsEmpty']
+
+  let hCount := cellEmptyCountOfIsEmpty hIsEmpty
+  simp [Nat.sub_add_cancel hCount]
+
+theorem newBoardIsFullAfterTurn8
+  (state : TicTacToeState)
+  (newState : TicTacToeState)
+  (pos : Position)
+  (_ : state.status = GameStatus.InProgress)
+  (hIsEmpty : isEmptyPosition state.board pos)
+  (_ : wellFormedGame state)
+  (hNewBoard : newState.board = Vector.set state.board pos.val (Cell.Occupied (currentPlayer state)))
+  : isBoardFull newState.board = (turnNumber state == 8) := by
+
+  let hAtLeastOneEmpty := hBoardNotFullIfCellEmpty state pos hIsEmpty
+  simp [isBoardFull] at hAtLeastOneEmpty
+  let hAtLeastOneEmpty := Nat.pos_of_ne_zero hAtLeastOneEmpty
+
+  simp [isBoardFull, turnNumber]
+  by_cases h : Vector.count Cell.Empty newState.board == 0
+  .
+    simp [h]
+
+    let hMoveDecrementsEmptyCellCount := moveDecrementsEmptyCellCount state newState pos hIsEmpty hNewBoard
+    let hMoveDecrementsEmptyCellCount := congrArg (· - 1) hMoveDecrementsEmptyCellCount
+    simp at hMoveDecrementsEmptyCellCount
+    simp [hMoveDecrementsEmptyCellCount] at h
+    let h := congrArg (· + 1) h
+    simp only at h
+
+    simp [Nat.sub_add_cancel hAtLeastOneEmpty] at h
+    simp [h]
+  .
+    simp [h]
+    simp at h
+
+    let h' := Nat.pos_of_ne_zero h
+    let hMoveDecrementsEmptyCellCount := moveDecrementsEmptyCellCount state newState pos hIsEmpty hNewBoard
+    let hMoveDecrementsEmptyCellCount := congrArg (· - 1) hMoveDecrementsEmptyCellCount
+    simp at hMoveDecrementsEmptyCellCount
+    simp [hMoveDecrementsEmptyCellCount] at h'
+
+    let h' := Nat.add_lt_add_right h' 9
+    simp only [Nat.zero_add] at h'
+
+    have hTrivial : state.board.count Cell.Empty ≤ 9 := Vector.count_le_size
+    let h' := Nat.sub_lt_sub_right hTrivial h'
+
+    have hSimplify : Vector.count Cell.Empty state.board - 1 + 9 - Vector.count Cell.Empty state.board = 8 := by
+      -- Swap (· - 1 + 9) to (· + 9 - 1) so it simplifies
+      let hCount := cellEmptyCountOfIsEmpty hIsEmpty
+      simp [← Nat.sub_add_comm hCount (m := 9)]
+
+    simp [hSimplify] at h'
+
+    let hNotEquals := (Iff.mp Nat.lt_iff_le_and_ne h').right
+    simp at hNotEquals
+    exact hNotEquals
+
+theorem noWinnersWhileInProgress
+  (state : TicTacToeState)
+  (hInProgress : state.status = GameStatus.InProgress)
+  (hWellFormed : wellFormedGame state)
+  : checkWin state.board Player.X = false ∧ checkWin state.board Player.O = false := by
+  simp [wellFormedGame, hInProgress] at hWellFormed
+  simp [hWellFormed]
+
+theorem singleWinner
+  (state : TicTacToeState)
+  (hWon : state.status = GameStatus.Won winner)
+  (hWellFormed : wellFormedGame state)
+  : checkWin state.board (switchPlayer winner) = false := by
+  simp [wellFormedGame, hWon] at hWellFormed
+  simp [hWellFormed]
+
+theorem playerXCellCount
+  (state : TicTacToeState)
+  (hWellFormed : wellFormedGame state)
+  : countMarkedCells state.board Player.X = (turnNumber state + 1 ) / 2 := by
+  let hWellFormed' := hWellFormed
+  simp [countMarkedCells, turnNumber]
+
+  have playerCellCount
+    : countMarkedCells state.board Player.X + countMarkedCells state.board Player.O = 9 - Vector.count Cell.Empty state.board := by
+    simp [countMarkedCells, Vector.count_eq_countP]
+
+    have hDisjoint : ∀ a, (a == Cell.Occupied Player.X -> ¬(a == Cell.Occupied Player.O)) ∧ (a == Cell.Occupied Player.O -> ¬(a == Cell.Occupied Player.X)) := by
+      intro a
+      match a with
+      | Cell.Empty => trivial
+      | Cell.Occupied Player.X => trivial
+      | Cell.Occupied Player.O => trivial
+
+    have hDisjoint' : ∀ a, (a == Cell.Occupied Player.X || a == Cell.Occupied Player.O) != (a == Cell.Empty) := by
+      intro a
+      match a with
+      | Cell.Empty => trivial
+      | Cell.Occupied Player.X => trivial
+      | Cell.Occupied Player.O => trivial
+
+    have hComplete : ∀ a, a == Cell.Occupied Player.X || a == Cell.Occupied Player.O || a == Cell.Empty := by
+      intro a
+      match a with
+      | Cell.Empty => trivial
+      | Cell.Occupied Player.X => trivial
+      | Cell.Occupied Player.O => trivial
+
+    simp [countDisjoint (xs := state.board) (pred1 := (fun x => x == Cell.Occupied Player.X)) (pred2 := (fun x => x == Cell.Occupied Player.O)) hDisjoint]
+    let hCountComplete := countComplete (xs := state.board) (pred1 := fun x => x == Cell.Occupied Player.X || x == Cell.Occupied Player.O) (pred2 := fun x => x == Cell.Empty) hDisjoint' hComplete
+    simp [Vector.size] at hCountComplete
+    simp [← hCountComplete]
+
+  simp [← playerCellCount]
+  match hStatus : state.status with
+  | GameStatus.Draw =>
+    simp [wellFormedGame, hStatus] at hWellFormed
+    simp [hWellFormed]
+    rw [← countMarkedCells]
+    simp [hWellFormed]
+  | GameStatus.InProgress =>
+    simp [wellFormedGame, hStatus] at hWellFormed
+    match hCurrentPlayer : currentPlayer state with
+    | Player.X =>
+      simp [hCurrentPlayer] at hWellFormed
+      simp [hWellFormed, ← Nat.two_mul, Nat.add_div (a := 2 * countMarkedCells state.board Player.X) (b := 1) (c := 2) (by trivial)]
+      simp [countMarkedCells]
+    | Player.O =>
+      simp [hCurrentPlayer] at hWellFormed
+      simp [
+        Nat.add_assoc,
+        hWellFormed,
+        ← Nat.two_mul,
+      ]
+      simp [countMarkedCells]
+  | GameStatus.Won winner =>
+    simp [wellFormedGame, hStatus] at hWellFormed
+    let hSingleWinner := singleWinner state hStatus hWellFormed'
+    simp [hSingleWinner] at hWellFormed
+    match winner with
+    | Player.X =>
+      simp at hWellFormed
+      simp [Nat.add_assoc, hWellFormed, ← Nat.two_mul]
+      simp [countMarkedCells]
+    | Player.O =>
+      simp at hWellFormed
+      simp [
+        ← hWellFormed,
+        ← Nat.two_mul,
+        Nat.add_div (a := 2 * countMarkedCells state.board Player.O) (b := 1) (c := 2) (by trivial)
+      ]
+      simp [hWellFormed]
+      simp [countMarkedCells]
+
 theorem makeMovePreservesWellFormedness
   {state : TicTacToeState}
-  {currentPlayer : Player}
   {pos : Position}
-  {hInProgress : state.status = GameStatus.InProgress currentPlayer}
+  {hInProgress : state.status = GameStatus.InProgress}
   {hIsEmpty : isEmptyPosition state.board pos}
   {hWellFormed : wellFormedGame state}
   : wellFormedGame (makeMove state pos hInProgress hIsEmpty hWellFormed) := by
+  let player := currentPlayer state
+  let hPlayer : player = currentPlayer state := by trivial
   let newState := (makeMove state pos hInProgress hIsEmpty hWellFormed)
   let newBoard := newState.board
-  have hNewBoard : newBoard = Vector.set state.board pos.val (Cell.Occupied currentPlayer) := by
+  have hNewBoard : newBoard = Vector.set state.board pos.val (Cell.Occupied player) := by
+    trivial
+  have hNewBoard' : newBoard = newState.board := by
     trivial
 
-  have hNoWinnersYet : checkWin state.board currentPlayer = false ∧ checkWin state.board (switchPlayer currentPlayer) = false := by
-    unfold wellFormedGame at hWellFormed
-    simp [hInProgress] at hWellFormed
-    match currentPlayer with
+  let hWellFormed' := hWellFormed
+  simp [wellFormedGame, hInProgress] at hWellFormed
+
+  have hNoWinnersYet : checkWin state.board player = false ∧ checkWin state.board (switchPlayer player) = false := by
+    match player with
     | Player.X => simp [switchPlayer, hWellFormed]
     | Player.O => simp [switchPlayer, hWellFormed]
 
-  simp [wellFormedGame, hInProgress] at hWellFormed
-  simp [makeMove]
+  let pMarkedO := fun x => x == Cell.Occupied Player.O
+  let pMarkedX := fun x => x == Cell.Occupied Player.X
+  let hIsEmpty' := hIsEmpty
+  simp [isEmptyPosition, Vector.get] at hIsEmpty'
+  let hNotMarkedO : ¬pMarkedO (state.board.get pos) := by
+    simp [pMarkedO, Vector.get, hIsEmpty']
+  let hNotMarkedX : ¬pMarkedX (state.board.get pos) := by
+    simp [pMarkedX, Vector.get, hIsEmpty']
 
-  match hMatch : (checkWin newBoard currentPlayer, checkWin newBoard (switchPlayer currentPlayer)) with
+  let xMarksUntouched := vector_count_set_other (i := pos) (xs := state.board) (pred := pMarkedO) (value := Cell.Occupied Player.X) (hOld := (by trivial)) (hNew := (by trivial))
+  let oMarksUntouched := vector_count_set_other (i := pos) (xs := state.board) (pred := pMarkedX) (value := Cell.Occupied Player.O) (hOld := (by trivial)) (hNew := (by trivial))
+  let xMarksIncreasedByOne := vector_count_set (i := pos) (xs := state.board) (pred := pMarkedX) (value := Cell.Occupied Player.X) (hOld := (by trivial)) (hNew := (by trivial))
+  let oMarksIncreasedByOne := vector_count_set (i := pos) (xs := state.board) (pred := pMarkedO) (value := Cell.Occupied Player.O) (hOld := (by trivial)) (hNew := (by trivial))
+  simp [pMarkedO] at xMarksUntouched
+  simp [pMarkedX] at xMarksIncreasedByOne
+  simp [pMarkedX] at oMarksUntouched
+  simp [pMarkedO] at oMarksIncreasedByOne
+
+  rw [makeMove, wellFormedGame, ← hNewBoard]
+  simp
+  let hPreviousCellCount := hWellFormed.right
+
+  -- State-specific properties
+  match hMatch : (checkWin newBoard player, checkWin newBoard (switchPlayer player)) with
   | (true, false) =>
     -- We have a winner!
     let hWonLeft := congrArg (fun x => x.1) hMatch
     simp at hWonLeft
     let hWonRight := congrArg (fun x => x.2) hMatch
     simp at hWonRight
-    simp [wellFormedGame, ← hNewBoard, hWonLeft, hWonRight]
+    simp [← hPlayer, hWonLeft, hWonRight]
+
+    -- The cell distribution is well formed
+    simp [hNewBoard]
+    match hCurrentPlayer : player with
+    | Player.X =>
+      simp [← hPlayer, hCurrentPlayer, countMarkedCells] at hPreviousCellCount
+      simp [
+        countMarkedCells,
+        xMarksUntouched,
+        congrArg (· + 1) hPreviousCellCount,
+        xMarksIncreasedByOne
+      ]
+    | Player.O =>
+      simp [← hPlayer, hCurrentPlayer, countMarkedCells] at hPreviousCellCount
+      simp [
+        countMarkedCells,
+        oMarksUntouched,
+        ← hPreviousCellCount,
+        oMarksIncreasedByOne
+      ]
   | (false, false) =>
     let hWonLeft := congrArg (fun x => x.1) hMatch
     simp at hWonLeft
     let hWonRight := congrArg (fun x => x.2) hMatch
     simp at hWonRight
-    simp [wellFormedGame, ← hNewBoard, hWonLeft]
+    simp [← hPlayer, hWonLeft]
+
     by_cases hDraw : isBoardFull newBoard
     . -- Draw
       simp [hDraw]
-      match hCurrentPlayer : currentPlayer with
-      | Player.X =>
-        simp [hCurrentPlayer] at hWonLeft
-        simp [switchPlayer, hCurrentPlayer] at hWonRight
-        simp [hWonLeft, hWonRight]
-      | Player.O =>
-        simp [hCurrentPlayer] at hWonLeft
-        simp [switchPlayer, hCurrentPlayer] at hWonRight
-        simp [hWonLeft, hWonRight]
+
+      -- We know player = Player.X, since they will always have the last turn
+      let hDrawAfterEigthTurn := newBoardIsFullAfterTurn8 state newState pos hInProgress hIsEmpty hWellFormed' hNewBoard
+      conv at hDrawAfterEigthTurn =>
+        pattern newState.board
+        change newBoard
+      simp [hDraw] at hDrawAfterEigthTurn
+      simp [← hPlayer] at hPreviousCellCount
+      simp [currentPlayer, hDrawAfterEigthTurn] at hPlayer
+      simp [hPlayer, countMarkedCells] at hPreviousCellCount
+
+      simp [hPlayer] at hWonLeft
+      simp [switchPlayer, hPlayer] at hWonRight
+      simp [hWonLeft, hWonRight]
+
+      -- Well-formed cell distribution
+      simp [
+        countMarkedCells,
+        hNewBoard,
+        hPlayer,
+        xMarksUntouched,
+        hPreviousCellCount,
+        xMarksIncreasedByOne
+      ]
+
+      -- We know Player.X has 4 cells at the beginning of move 8
+      let hPlayerXHas4Cells := playerXCellCount state hWellFormed'
+      simp [hDrawAfterEigthTurn] at hPlayerXHas4Cells
+      rw [← countMarkedCells, hPlayerXHas4Cells]
+
     . -- The game goes on
       simp [hDraw]
-      match hCurrentPlayer : currentPlayer with
+
+      have hNoWinners : checkWin newBoard Player.X = false ∧ checkWin newBoard Player.O = false := by
+        match hPlayerToCheck : player with
+        | Player.X =>
+            simp [hPlayerToCheck] at hWonLeft
+            simp [hPlayerToCheck, switchPlayer] at hWonRight
+            simp [hWonLeft, hWonRight]
+        | Player.O =>
+            simp [hPlayerToCheck] at hWonLeft
+            simp [hPlayerToCheck, switchPlayer] at hWonRight
+            simp [hWonLeft, hWonRight]
+
+      have modLemma {x : Nat} : (x % 2 = 0) = ((x + 1) % 2 = 1) := by
+        simp
+        by_cases hCase : x % 2 = 0
+        . simp at hCase
+          simp [hCase, Nat.add_mod]
+        . simp at hCase
+          simp [hCase]
+          simp [← hCase, ← Nat.two_mul]
+
+      have hNextPlayer : currentPlayer newState = switchPlayer (currentPlayer state) := by
+        simp [currentPlayer, switchPlayer]
+        let hTurnNumber := moveIncrementsTurnNumber state newState pos hIsEmpty hNewBoard
+        let hModLemma := modLemma (x := turnNumber state)
+        by_cases hIf : turnNumber newState % 2 = 0
+        . simp [hIf]
+          simp [hModLemma, ← hTurnNumber, hIf]
+        . simp at hIf
+          simp [hIf]
+          simp [hModLemma, ← hTurnNumber, hIf]
+
+      simp [hNoWinners]
+      match hCurrentPlayer : player with
       | Player.X =>
-        simp [hCurrentPlayer] at hWonLeft
-        simp [switchPlayer, hCurrentPlayer] at hWonRight
-        simp [hWonLeft, hWonRight]
+        rw [hPlayer] at hCurrentPlayer
+        conv =>
+          pattern currentPlayer { board := newBoard, status := GameStatus.InProgress }
+          change currentPlayer newState
+        conv =>
+          pattern currentPlayer { board := newBoard, status := GameStatus.InProgress }
+          change currentPlayer newState
+        simp [hNextPlayer, hCurrentPlayer, switchPlayer]
+        simp [noWinnersWhileInProgress state hInProgress hWellFormed', hCurrentPlayer] at hWellFormed
+        simp [hNewBoard, countMarkedCells, xMarksUntouched]
+        rw [← countMarkedCells]
+        simp [hWellFormed]
+        simp [countMarkedCells, xMarksIncreasedByOne]
       | Player.O =>
-        simp [hCurrentPlayer] at hWonLeft
-        simp [switchPlayer, hCurrentPlayer] at hWonRight
-        simp [hWonLeft, hWonRight]
+        rw [hPlayer] at hCurrentPlayer
+        conv =>
+          pattern currentPlayer { board := newBoard, status := GameStatus.InProgress }
+          change currentPlayer newState
+        conv =>
+          pattern currentPlayer { board := newBoard, status := GameStatus.InProgress }
+          change currentPlayer newState
+        simp [hNextPlayer, hCurrentPlayer, switchPlayer]
+        simp [noWinnersWhileInProgress state hInProgress hWellFormed', hCurrentPlayer] at hWellFormed
+        simp [hNewBoard, countMarkedCells, oMarksUntouched]
+        rw [← countMarkedCells, ← countMarkedCells]
+        simp [← hWellFormed]
+        simp [countMarkedCells, oMarksIncreasedByOne]
   | (_, true) =>
     -- This branch is unreachable, so the known facts at this point must lead to a contradiction.
     let hWonLeft := congrArg (fun x => x.1) hMatch
@@ -338,71 +796,45 @@ theorem makeMovePreservesWellFormedness
 
     -- If the other player already won, it must have won before the last move, which
     -- is impossible (it would mean the game state was not well formed at the last move)
-    let hNoPreviousWinner := noWinWithoutOwnMove state.board (switchPlayer currentPlayer) pos hIsEmpty hNoWinnersYet.right
+    let hNoPreviousWinner := noWinWithoutOwnMove state.board (switchPlayer player) pos hIsEmpty hNoWinnersYet.right
     simp [switchPlayerIdentity, ← hNewBoard] at hNoPreviousWinner
     simp [hNoPreviousWinner] at hWonRight
 
 -- Proof: players alternate after each move
 theorem playersAlternateAfterMove
   {state : TicTacToeState}
-  {currentPlayer : Player}
   {pos : Position}
-  {hInProgress : state.status = GameStatus.InProgress currentPlayer}
+  {hInProgress : state.status = GameStatus.InProgress}
   {hIsEmpty : isEmptyPosition state.board pos}
   {hWellFormed : wellFormedGame state}
   {newState : TicTacToeState}
-  (
-    h: makeMove state pos hInProgress hIsEmpty hWellFormed = newState
-  ) : (
-    newState.status = GameStatus.InProgress (switchPlayer currentPlayer) ∨
-    newState.status = GameStatus.Won currentPlayer ∨
-    newState.status = GameStatus.Draw
-  ) := by
-  let h' := congrArg (fun x : TicTacToeState => x.status) h
-  simp at h'
-  rw [Eq.symm h']
-
-  match hMatch : (makeMove state pos hInProgress hIsEmpty hWellFormed).status with
-  | GameStatus.Won winner =>
-    -- Get ourselves a clear goal
-    right
-    left
-    simp
-
-    -- Now work towards it
-    rw [h] at hMatch
-    unfold makeMove at h'
-    rw [hMatch] at h'
-    grind
-  | GameStatus.InProgress nextPlayer =>
-    -- Get ourselves a clear goal
-    left
-    simp
-
-    -- Now work towards it
-    rw [h] at hMatch
-    unfold makeMove at h'
-    rw [hMatch] at h'
-    grind
-  | GameStatus.Draw =>
-    right
-    right
-    simp
+  (hNewState: newState = makeMove state pos hInProgress hIsEmpty hWellFormed)
+  : currentPlayer state = switchPlayer (currentPlayer newState) := by
+  let hNewBoard := congrArg (fun s => s.board) hNewState
+  simp at hNewBoard
+  let hMoveIncrementsTurnNumber := moveIncrementsTurnNumber state newState pos hIsEmpty hNewBoard
+  simp [currentPlayer, hMoveIncrementsTurnNumber]
+  by_cases hCase : turnNumber state % 2 = 0
+  . simp [hCase]
+    have hNextTurnNumber : (turnNumber state + 1) % 2 = 1 := by
+      simp [Nat.add_mod, hCase]
+    simp [hNextTurnNumber, switchPlayer]
+  . simp at hCase
+    simp [hCase]
+    have hNextTurnNumber : (turnNumber state + 1) % 2 = 0 := by
+      simp [Nat.add_mod, hCase]
+    simp [hNextTurnNumber, switchPlayer]
 
 -- Proof: cell gets marked after move with the player's mark
 theorem cellMarkedAfterMove
   {state : TicTacToeState}
-  {currentPlayer : Player}
   {pos : Position}
-  {hInProgress : state.status = GameStatus.InProgress currentPlayer}
+  {hInProgress : state.status = GameStatus.InProgress}
   {hIsEmpty : isEmptyPosition state.board pos}
   {hWellFormed : wellFormedGame state}
   {newState : TicTacToeState}
-  (
-    h: makeMove state pos hInProgress hIsEmpty hWellFormed = newState
-  ) : (
-    newState.board.get pos = Cell.Occupied currentPlayer
-  ) := by
+  (h: makeMove state pos hInProgress hIsEmpty hWellFormed = newState)
+  : newState.board.get pos = Cell.Occupied (currentPlayer state) := by
   unfold makeMove at h
   let h' := congrArg (fun x : TicTacToeState => x.board) h
   simp at h'
